src/cbor/pulse/raw/everparse/CBOR.Pulse.Raw.EverParse.Det.Impl.Aux.fst
@@ -1,0 +1,70 @@
+module CBOR.Pulse.Raw.EverParse.Det.Impl.Aux
+friend CBOR.Spec.API.Format
+
+module Spec = CBOR.Spec.API.Format
+module SpecRawBase = CBOR.Spec.Raw.Base
+module SpecRaw = CBOR.Spec.Raw
+module Optimal = CBOR.Spec.Raw.Optimal
+module Format = CBOR.Spec.Raw.Format
+
+let mk_det_raw_cbor_tot (c: Spec.cbor) : Tot SpecRawBase.raw_data_item
+= SpecRaw.mk_det_raw_cbor c
+
+let det_raw_list (l: list Spec.cbor) : Tot (list SpecRawBase.raw_data_item)
+= List.Tot.map mk_det_raw_cbor_tot l
+
+#push-options "--fuel 1 --ifuel 1 --z3rlimit 32"
+
+let rec list_map_mk_det_raw_cbor_correct (l: list Spec.cbor)
+: Lemma (ensures (
+    let l' = det_raw_list l in
+    List.Tot.for_all Optimal.raw_data_item_ints_optimal l' /\
+    List.Tot.for_all (Optimal.raw_data_item_sorted Format.deterministically_encoded_cbor_map_key_order) l'
+  ))
+= match l with
+  | [] -> ()
+  | _ :: q -> list_map_mk_det_raw_cbor_correct q
+
+let rec list_map_mk_cbor_mk_det_raw_cbor (l: list Spec.cbor)
+: Lemma (ensures (List.Tot.map SpecRaw.mk_cbor (det_raw_list l) == l))
+= match l with
+  | [] -> ()
+  | _ :: q -> list_map_mk_cbor_mk_det_raw_cbor q
+
+let rec mk_det_raw_cbor_inj_map (l1 l2: list Spec.cbor)
+: Lemma
+    (requires det_raw_list l1 == det_raw_list l2)
+    (ensures l1 == l2)
+    (decreases l1)
+= match l1, l2 with
+  | [], [] -> ()
+  | x1 :: t1, x2 :: t2 ->
+    SpecRaw.mk_det_raw_cbor_inj x1 x2;
+    mk_det_raw_cbor_inj_map t1 t2
+
+let length_det_raw_list (l: list Spec.cbor)
+  : Lemma (List.Tot.length (det_raw_list l) == List.Tot.length l)
+          [SMTPat (List.Tot.length (det_raw_list l))]
+= ()
+
+(* Lemma: when y is a det cbor that unpacks to CArray l, then mk_det_raw_cbor y is Array _ (det_raw_list l) *)
+let mk_det_raw_cbor_array_eq (y: Spec.cbor) (l: list Spec.cbor)
+: Lemma
+    (requires
+      FStar.UInt.fits (List.Tot.length l) 64 /\
+      Spec.unpack y == Spec.CArray l)
+    (ensures
+       SpecRawBase.Array? (SpecRaw.mk_det_raw_cbor y) /\
+       (SpecRawBase.Array?.v (SpecRaw.mk_det_raw_cbor y) <: list SpecRawBase.raw_data_item) == det_raw_list l)
+= Spec.pack_unpack y;
+  let len = Optimal.mk_raw_uint64 (FStar.UInt64.uint_to_t (List.Tot.length l)) in
+  let l' = det_raw_list l in
+  let x : SpecRawBase.raw_data_item = SpecRawBase.Array len l' in
+  list_map_mk_cbor_mk_det_raw_cbor l;
+  list_map_mk_det_raw_cbor_correct l;
+  Optimal.raw_data_item_sorted_optimal_valid Format.deterministically_encoded_cbor_map_key_order x;
+  SpecRaw.mk_cbor_eq x;
+  SpecRaw.mk_det_raw_cbor_mk_cbor x;
+  assert (SpecRaw.mk_det_raw_cbor (Spec.pack (Spec.CArray l)) == x)
+
+#pop-options
