src/cbor/pulse/raw/everparse/CBOR.Pulse.Raw.EverParse.Det.Impl.Aux.fsti
@@ -1,0 +1,27 @@
+module CBOR.Pulse.Raw.EverParse.Det.Impl.Aux
+
+module Spec = CBOR.Spec.API.Format
+module SpecRawBase = CBOR.Spec.Raw.Base
+module SpecRaw = CBOR.Spec.Raw
+
+val mk_det_raw_cbor_tot (c: Spec.cbor) : Tot SpecRawBase.raw_data_item
+
+val det_raw_list (l: list Spec.cbor) : Tot (list SpecRawBase.raw_data_item)
+
+val mk_det_raw_cbor_inj_map (l1 l2: list Spec.cbor)
+: Lemma
+    (requires det_raw_list l1 == det_raw_list l2)
+    (ensures l1 == l2)
+
+val length_det_raw_list (l: list Spec.cbor)
+  : Lemma (List.Tot.length (det_raw_list l) == List.Tot.length l)
+          [SMTPat (List.Tot.length (det_raw_list l))]
+
+val mk_det_raw_cbor_array_eq (y: Spec.cbor) (l: list Spec.cbor)
+: Lemma
+    (requires
+      FStar.UInt.fits (List.Tot.length l) 64 /\
+      Spec.unpack y == Spec.CArray l)
+    (ensures
+       SpecRawBase.Array? (SpecRaw.mk_det_raw_cbor y) /\
+       (SpecRawBase.Array?.v (SpecRaw.mk_det_raw_cbor y) <: list SpecRawBase.raw_data_item) == det_raw_list l)
